theories/typing/array_util.v
@@ -4,6 +4,9 @@ Set Default Proof Using "Type".
 Notation "l +ₗ[ ty ] i" := (l%L +ₗ Z.of_nat (i%nat * ty.(ty_size))%nat)
   (format "l  +ₗ[ ty ]  i", at level 50, left associativity) : loc_scope.
 
+Notation "l ↦∗len n" := (∃vl, ⌜length vl = n%nat⌝ ∗ l ↦∗ vl)%I
+  (at level 20, format "l  ↦∗len  n") : bi_scope.
+
 Section array_util.
   Context `{!typeG Σ}.
 
@@ -67,4 +70,15 @@ Section array_util.
     iMod ("Toty" with "ξl") as "[$$]". by iMod ("Totys" with "ζl") as "[$$]".
   Qed.
 
+  Lemma leak_mt_big_sepL {𝔄} (ty: type 𝔄) n (aπl: vec _ n) d tid l :
+    ([∗ list] i ↦ aπ ∈ aπl, (l +ₗ[ty] i) ↦∗: ty.(ty_own) aπ d tid)%I ⊢
+    l ↦∗len (n * ty.(ty_size)).
+  Proof.
+    iInduction aπl as [|] "IH" forall (l)=>/=.
+    { iIntros. iExists []. by rewrite heap_mapsto_vec_nil. }
+    iIntros "((%& ↦ & ty) & ↦tys)". rewrite ty_size_eq. iDestruct "ty" as %Eq.
+    setoid_rewrite <-shift_loc_assoc_nat. iDestruct ("IH" with "↦tys") as "(%&%& ↦')".
+    iExists (_++_). rewrite app_length heap_mapsto_vec_app shift_loc_0 -{3}Eq.
+    iFrame "↦ ↦'". iPureIntro. by f_equal.
+  Qed.
 End array_util.
